Work on proving analysis correct

extraction/theories/AnalyzeCorrectness.v
@@ -13,6 +13,14 @@ Import ListNotations.
 Import ExAst.
 Open Scope bool.
 
+Lemma get_mib_masks_eq kn mm im :
+  get_mib_masks ((kn, mm) :: im) kn = Some mm.
+Proof.
+  unfold get_mib_masks.
+  cbn.
+  now rewrite eq_kername_refl.
+Qed.
+
 Lemma get_mib_masks_ne p im kn :
   fst p <> kn ->
   get_mib_masks (p :: im) kn = get_mib_masks im kn.
@@ -22,6 +30,14 @@ Proof.
   destruct p; cbn in *.
   unfold eq_kername.
   now destruct (kername_eq_dec _ _).
+Qed.
+
+Lemma get_const_mask_eq kn mask cm :
+  get_const_mask ((kn, mask) :: cm) kn = mask.
+Proof.
+  unfold get_const_mask.
+  cbn.
+  now rewrite eq_kername_refl.
 Qed.
 
 Lemma valid_case_masks_add_new Σ kn brs im ind npars m :
@@ -86,7 +102,7 @@ Proof.
     now rewrite H.
 Qed.
 
-Lemma valid_masks_decl_add_new Σ kn im cm m :
+Lemma valid_masks_decl_add_ind Σ kn im cm m :
   lookup_env Σ kn = None ->
   wfe_env Σ ->
   valid_masks_env im cm Σ ->
@@ -106,7 +122,543 @@ Proof.
   now eapply valid_cases_add_new.
 Qed.
 
-Lemma analyze_correct Σ :
+Lemma valid_masks_decl_add_const Σ kn im cm mask :
+  lookup_env Σ kn = None ->
+  wfe_env Σ ->
+  valid_masks_env im cm Σ ->
+  forallb (valid_masks_decl im ((kn, mask) :: cm)) Σ.
+Proof.
+  intros no_prev wfe valid.
+  induction Σ as [|(kn', decl) Σ IH]; [easy|].
+  cbn in *.
+  unfold eq_kername in no_prev.
+  destruct (kername_eq_dec _ _); [easy|].
+  destruct decl; cbn in *; propify; [|easy|easy].
+  destruct c.
+  destruct cst_body; cbn in *; [|easy].
+  propify.
+  split; [|easy].
+  split; [|easy].
+  Admitted.
+
+Lemma nth_clear_bit_eq k bs :
+  nth k (clear_bit k bs) false = false.
+Proof.
+  revert bs.
+  induction k as [|k IH]; intros bs; cbn in *.
+  - now destruct bs.
+  - now destruct bs.
+Qed.
+
+Lemma nth_clear_bit_neq k k' bs :
+  k <> k' ->
+  nth k (clear_bit k' bs) false = nth k bs false.
+Proof.
+  revert bs k'.
+  induction k as [|k IH]; intros bs k' ne.
+  - destruct k'; [easy|].
+    now destruct bs.
+  - destruct k'.
+    + destruct bs; [|easy].
+      now destruct k.
+    + destruct bs; [easy|].
+      cbn.
+      now apply IH.
+Qed.
+
+Lemma hd_nth {A} d (l : list A) :
+  hd d l = nth 0 l d.
+Proof. now destruct l. Qed.
+
+Lemma nth_tl {A} k (l : list A) d :
+  nth k (tl l) d = nth (S k) l d.
+Proof.
+  destruct l.
+  - now destruct k.
+  - easy.
+Qed.
+
+Lemma analyze_top_level_analyze state n t :
+  analyze_top_level analyze state n t =
+  ((analyze_top_level analyze state n t).1, analyze state t).
+Proof.
+  induction t in state, n |- * using term_forall_list_ind; cbn in *; auto.
+  - destruct n; [easy|].
+    destruct analyze_top_level eqn:an.
+    rewrite IHt in an.
+    now noconf an.
+  - destruct analyze_top_level eqn:an.
+    rewrite IHt2 in an.
+    now noconf an.
+Qed.
+
+Definition consistent_mib_mask (mm : mib_masks) (mib : mutual_inductive_body) : Prop :=
+  (#|param_mask mm| = ind_npars mib) /\
+  ∥Alli (fun ind oib =>
+           Alli (fun c '(_, args) => #|get_branch_mask mm ind c| = #|args|)
+                0
+                (ind_ctors oib))
+   0
+   (ind_bodies mib)∥.
+
+Definition consistent_mib_masks (Σ : global_env) (im : list (kername × mib_masks)) : Prop :=
+  forall kn,
+    match lookup_minductive Σ kn with
+    | Some mib =>
+      match get_mib_masks im kn with
+      | Some mm => consistent_mib_mask mm mib
+      | None => False
+      end
+    | None => True
+    end.
+
+Lemma get_mib_masks_update_eq im kn mm' mm :
+  get_mib_masks im kn = Some mm' ->
+  get_mib_masks (update_mib_masks kn mm im) kn = Some mm.
+Proof.
+  intros ex.
+  induction im as [|(kn', mm'') im IH]; [easy|].
+  cbn in *.
+  unfold eq_kername.
+  destruct (kername_eq_dec kn' kn) as [->|].
+  - now rewrite get_mib_masks_eq.
+  - now rewrite get_mib_masks_ne in * by easy.
+Qed.
+
+Lemma get_mib_masks_update_neq kn mm im kn' :
+  kn' <> kn ->
+  get_mib_masks (update_mib_masks kn mm im) kn' = get_mib_masks im kn'.
+Proof.
+  intros ne.
+  induction im as [|(kn'', mm') im IH]; [easy|].
+  cbn in *.
+  unfold eq_kername.
+  destruct (kername_eq_dec kn'' kn) as [->|].
+  - now rewrite !get_mib_masks_ne in * by easy.
+  - unfold get_mib_masks.
+    cbn.
+    unfold eq_kername.
+    now destruct (kername_eq_dec kn'' kn'); [congruence|].
+Qed.
+
+Lemma consistent_mib_masks_update Σ im kn mm mib :
+  consistent_mib_masks Σ im ->
+  consistent_mib_mask mm mib ->
+  lookup_minductive Σ kn = Some mib ->
+  consistent_mib_masks Σ (update_mib_masks kn mm im).
+Proof.
+  intros cons_mms cons_mm found kn'.
+  destruct (eq_dec kn kn') as [<-|].
+  - specialize (cons_mms kn).
+    rewrite found in *.
+    destruct get_mib_masks eqn:mmeq in cons_mms; [|easy].
+    now erewrite get_mib_masks_update_eq by eassumption.
+  - specialize (cons_mms kn').
+    destruct lookup_minductive; [|easy].
+    now rewrite get_mib_masks_update_neq by easy.
+Qed.
+
+Lemma mib_masks_consistent_analyze Σ t state :
+  wfe_term Σ t ->
+  consistent_mib_masks Σ state.2 ->
+  consistent_mib_masks Σ (analyze state t).2.
+Proof.
+  intros wf_t cons_mm.
+  induction t in state, wf_t, cons_mm |- * using term_forall_list_ind; cbn in *; auto.
+  - induction H; [easy|].
+    cbn in *.
+    now propify.
+  - propify.
+    now apply IHt2, IHt1.
+  - propify.
+    now apply IHt2, IHt1.
+  - destruct p.
+    propify.
+    destruct get_mib_masks eqn:mm; [|easy].
+    destruct analyze_case_branches eqn:an.
+    apply IHt in cons_mm; [|easy].
+    specialize (cons_mm (inductive_mind i)) as cons.
+    destruct lookup_minductive eqn:?; [|now propify].
+    rewrite mm in *.
+    cbn.
+    eapply consistent_mib_masks_update.
+    + admit.
+    + now destruct m0.
+    cbn.
+    eapply consistent_mib_masks_update. [easy| |eassumption].
+    induction X.
+    + cbn.
+      apply IHt in cons_mm; [|easy].
+      specialize (cons_mm (inductive_mind i)) as cons.
+      destruct lookup_minductive eqn:?; [|now propify].
+      rewrite mm in *.
+      eapply consistent_mib_masks_update; [easy| |eassumption].
+      now destruct m.
+    + cbn in *.
+      * apply IHt.
+      destruct get_mib_masks eqn:mm' in valid_im; [|easy].
+      propify.
+      destruct wf_t as ((<- & ?) & _).
+
+    easy.
+    easy.
+    apply H in valid_im.
+    easy.
+
+Lemma nth_analyze Σ t k state :
+  wfe_term Σ t ->
+  valid_ind_masks Σ state.2 ->
+  nth k (analyze state t).1 false = nth k state.1 false && is_dead k t.
+Proof.
+  intros wf_t valid_im.
+  induction t in k, state, wf_t, valid_im |- * using term_forall_list_ind; cbn in *; propify.
+  - now btauto.
+  - destruct (Nat.eqb_spec n k) as [<-|];
+      [rewrite nth_clear_bit_eq|rewrite nth_clear_bit_neq by easy];
+      btauto.
+  - now btauto.
+  - induction H; cbn in *; [now btauto|].
+    propify.
+    rewrite H, IHForall.
+    btauto.
+    easy.
+    easy.
+    now btauto.
+  - rewrite nth_tl, IHt by easy.
+    cbn.
+    now btauto.
+  - rewrite nth_tl, IHt2 by easy.
+    cbn.
+    rewrite IHt1 by easy.
+    now btauto.
+  - rewrite IHt2, IHt1 by easy.
+    now btauto.
+  - now btauto.
+  - now btauto.
+  - destruct p as (ind & npars).
+*)
+
+(*
+Lemma nth_analyze' t :
+  (forall k state n,
+      nth k (analyze_top_level analyze state n t).2.1 false = nth k state.1 false && is_dead k t) /\
+  (forall k state,
+      nth k (analyze state t).1 false = nth k state.1 false && is_dead k t).
+Proof.
+  induction t using term_forall_list_ind; cbn in *.
+  - now split; intros; btauto.
+  - split; intros.
+    + destruct (Nat.eqb_spec n k) as [<-|].
+      * rewrite nth_clear_bit_eq.
+        now btauto.
+      * rewrite nth_clear_bit_neq by easy.
+        now btauto.
+    + destruct (Nat.eqb_spec n k) as [<-|].
+      * rewrite nth_clear_bit_eq.
+        now btauto.
+      * rewrite nth_clear_bit_neq by easy.
+        now btauto.
+  - now split; intros; btauto.
+  - induction H; cbn in *; [now split; intros; btauto|].
+    destruct H.
+    destruct IHForall.
+    split; intros.
+    + rewrite H1, H2; [now btauto|exact 0].
+    + rewrite H1, H2; [now btauto|exact 0].
+  - destruct IHt.
+    split; intros.
+    + destruct n0; cbn.
+      * now rewrite nth_tl, H0.
+      * destruct analyze_top_level eqn:an.
+        unfold remove_var.
+        cbn.
+        rewrite nth_tl.
+        specialize (H (S k) (new_var state) n0).
+        rewrite an in H.
+        cbn in *.
+        now rewrite H.
+    + now rewrite nth_tl, H0.
+  - destruct IHt1, IHt2.
+    split; intros.
+    + destruct analyze_top_level eqn:an.
+      unfold remove_var.
+      cbn.
+      rewrite nth_tl.
+      specialize (H1 (S k) (new_var (analyze state t1)) n0).
+      rewrite an in H1.
+      cbn in *.
+      rewrite H1, H0.
+      now btauto.
+    + rewrite nth_tl, H2.
+      cbn.
+      rewrite H0.
+      now btauto.
+  - destruct IHt1, IHt2.
+    split; intros.
+    + rewrite H2, H0.
+      now btauto.
+    + rewrite H2, H0.
+      now btauto.
+  - now split; intros; btauto.
+  - now split; intros; btauto.
+  - destruct p, IHt.
+    split; intros.
+    + destruct get_mib_masks; cycle 1.
+      * rewrite H0.
+  - now split; intros; btauto.
+  - now split; intros; btauto.
+  - now split; intros; btauto.
+  - now split; intros; btauto.
+  -
+    + destruct analyze_top_level eqn:an.
+      unfold remove_var.
+      cbn.
+      rewrite nth_tl.
+      specialize (H1 (S k) (new_var (analyze state t1)) n0).
+      rewrite an in H1.
+      cbn in *.
+      rewrite H1, H0.
+      now btauto.
+    + rewrite nth_tl, H2.
+      cbn.
+      rewrite H0.
+      now btauto.
+      unfold new_var.
+      cbn.
+      easy.
+      now btauto
+        destruct k.
+        -- cbn.
+        rewrite hd_nth.
+  - now split; intros; btauto.
+  - now split; intros; btauto.
+  - now split; intros; btauto.
+  - now split; intros; btauto.
+  - now split; intros; btauto.
+  - now split; intros; btauto.
+  - now split; intros; btauto.
+  - now split; intros; btauto.
+    + destruct k.
+      cbn.
+*)
+
+(*
+Lemma analyze_correct' Σ t :
+  wfe_term Σ t ->
+  (forall Γ im n mask Γ' im',
+      analyze_top_level analyze (Γ, im) n t = (mask, (Γ', im')) ->
+      (Γ', im') = analyze (Γ, im) t /\ valid_dearg_mask mask t /\ valid_cases im' t) /\
+  (forall Γ im Γ' im',
+      analyze (Γ, im) t = (Γ', im') ->
+      (forall k, nth k Γ' false = nth k Γ false && is_dead k t) /\
+      (forall t', valid_cases im t' -> valid_cases im' t') /\ valid_cases im' t).
+Proof.
+  induction t using term_forall_list_ind; cbn in *.
+  - split; intros; noconf H; [easy|].
+    split; [|easy].
+    now intros; btauto.
+  - split; intros; noconf H; [easy|].
+    split; [|easy].
+    intros.
+    cbn.
+    destruct (Nat.eqb_spec n k) as [<-|].
+    + rewrite nth_clear_bit_eq.
+      now btauto.
+    + rewrite nth_clear_bit_neq by easy.
+      now btauto.
+  - split; intros; noconf H; [easy|].
+    split; [|easy].
+    intros; btauto.
+  - split; intros.
+    + noconf H0.
+      cbn.
+      split; [easy|].
+      split; [easy|].
+      induction H in Γ, im, Γ', im', H0 |- *; [easy|].
+      destruct H.
+      cbn in *.
+      destruct fold_right eqn:fr.
+      cbn in *; propify; split.
+      * now apply H2 in H0.
+      * apply IHForall in fr.
+        apply H2 in H0 as (_ & ? & _).
+        clear -H0 fr.
+        induction l; [easy|].
+        cbn in *; propify.
+        now rewrite H0, IHl by easy.
+    + induction H in Γ, im, Γ', im', H0 |- *; cbn in *;
+        [noconf H0; split; intros; auto; btauto|].
+      destruct H.
+      destruct fold_right eqn:fr.
+      apply IHForall in fr as (? & ?).
+      apply H2 in H0 as (? & ?).
+      split.
+      * intros.
+        rewrite H0, H3.
+        now btauto.
+      * propify.
+        intuition auto.
+        clear -H4 H7.
+        induction l; [easy|].
+        cbn in *; propify.
+        now rewrite H4, IHl.
+  - destruct IHt.
+    split; intros; cbn in *.
+    + destruct n0; cbn in *.
+      * noconf H1.
+        unfold new_var, remove_var; cbn in *.
+        split; [easy|].
+        split; [easy|].
+        destruct analyze eqn:an.
+        apply H0 in an.
+        easy.
+      * destruct analyze_top_level eqn:an.
+        noconf H1.
+        unfold new_var, remove_var in *; cbn in *.
+        destruct a; cbn in *.
+        apply H in an as (? & ?).
+        propify.
+        pattern (analyze (true :: Γ, im) t). (* wtf? *)
+        rewrite <- H1.
+        split; [easy|].
+        intuition auto.
+        destruct analyze eqn:an.
+        apply H0 in an.
+        intuition auto.
+        noconf H1.
+        specialize (H2 0).
+        cbn in *.
+        rewrite hd_nth.
+        rewrite H2.
+        now destruct ?.
+    + destruct analyze eqn:an.
+      apply H0 in an.
+      unfold remove_var in *.
+      cbn in *.
+      noconf H1.
+      intuition auto.
+      rewrite nth_tl.
+      rewrite H1.
+      now btauto.
+  - destruct IHt1, IHt2.
+    split; intros.
+    + unfold new_var, remove_var in *.
+
+      destruct analyze eqn:an.
+      apply H0 in an as (? & ?).
+
+      destruct analyze_top_level eqn:an.
+      cbn in *.
+      noconf H3.
+      destruct a.
+      apply H1 in an as (-> & ? & ?).
+      split; [easy|].
+      split; [easy|].
+
+      destruct analyze eqn:an.
+      apply H2 in an as (? & ?).
+      propify; intuition auto.
+    + unfold new_var, remove_var in *.
+      noconf H3; cbn in *.
+
+      destruct (analyze (Γ, im) t1) eqn:an.
+      cbn in *.
+      apply H0 in an as (? & ?).
+      destruct analyze eqn:an.
+      apply H2 in an as (? & ?).
+      cbn in *.
+      split.
+      * intros.
+        rewrite nth_tl, H5, H3.
+        now btauto.
+      * propify.
+        intuition auto.
+  - destruct IHt1, IHt2.
+    split; intros.
+    + noconf H3; cbn in *.
+      destruct (analyze (Γ, im) t1) eqn:an.
+      propify.
+      split; [easy|].
+      split; [easy|].
+      apply H0 in an as (? & ?).
+      apply H2 in H3 as (? & ?).
+      easy.
+    + destruct (analyze (Γ, im) t1) eqn:an.
+      propify.
+      apply H0 in an as (? & ?).
+      apply H2 in H3 as (? & ?).
+      intuition auto.
+      rewrite H3, H4.
+      now btauto.
+  - split; intros; noconf H; [easy|].
+    split; [|easy].
+    now intros; btauto.
+  - split; intros; noconf H; [easy|].
+    split; [|easy].
+    now intros; btauto.
+  - destruct IHt.
+    split; intros.
+    + destruct p.
+      destruct get_mib_masks; cycle 1.
+      { destruct analyze eqn:an.
+        noconf H1.
+        split; [easy|].
+        split; [easy|].
+        propify.
+        apply H0 in an as (? & ? & ?).
+        intuition auto.
+        admit.
+        admit. }
+      admit.
+    + admit.
+  - destruct s as ((ind & npars) & arg).
+    destruct IHt.
+    admit.
+  - split; intros.
+    + unfold new_vars, remove_vars in *; cbn in *.
+      noconf H0.
+      split; [easy|].
+      split; [easy|].
+      induction H in Γ, im |- *; [easy|].
+      cbn in *.
+
+Lemma analyze_top_level_correct Γ im n t mask Γ' im' :
+  analyze_top_level analyze (Γ, im) n t = (mask, (Γ', im')) ->
+  (Γ', im') = analyze (Γ, im) t /\ valid_dearg_mask mask t /\ valid_cases im' t.
+Proof.
+  intros an.
+  induction t in Γ, im, mask, Γ', im', an |- * using term_forall_list_ind;
+    cbn in *; try solve [now noconf an].
+  - noconf an.
+    rewrite H0.
+    split; [easy|].
+    split; [easy|].
+    induction H in Γ, im, H0 |- *; [easy|].
+    cbn in *.
+    propify; split.
+    +
+    induction l using List.rev_ind; [easy|].
+    rewrite fold_left_app in *.
+    cbn in *.
+    apply Forall_snoc in H as (? & ?).
+    rewrite forallb_app.
+    cbn; propify.
+    intuition auto.
+    +
+    apply and_assoc.
+    split; [|easy].
+    induction H; [easy|].
+    cbn in *.
+    propify; split; [|easy].
+  - noconf an.
+    cbn.
+    easy.
+  - noconf an.
+    easy.
+  -
+*)
+
+Lemma analyze_env_correct Σ :
   wfe_env Σ ->
   let (consts, inds) := analyze_env Σ in
   valid_masks_env inds consts Σ.
@@ -114,11 +666,20 @@ Proof.
   intros wfe.
   induction Σ as [|(kn, decl) Σ IH]; [easy|].
   cbn in *.
-  propify.
+  destruct lookup_env eqn:no_prev; [easy|].
+  cbn in *; propify.
   specialize (IH (proj2 wfe)).
   destruct (analyze_env Σ).
   destruct decl; cycle 1; cbn.
-  - destruct lookup_env eqn:no_prev; [easy|].
-    now apply valid_masks_decl_add_new.
+  - now apply valid_masks_decl_add_ind.
   - easy.
-  -
+  - destruct analyze_constant eqn:an.
+    propify.
+    split.
+    + destruct c, cst_body; [|easy].
+      rewrite get_const_mask_eq.
+      propify.
+      cbn in *.
+Lemma analyze_correct :
+    + apply valid_masks_decl_add_const; [easy|easy|].
+      admit.
